src/Assembly/Pseudize.v
@@ -1,0 +1,184 @@
+Require Export Bedrock.Word Bedrock.Nomega.
+Require Import NArith NPeano List Sumbool.
+Require Import QhasmCommon QhasmEvalCommon QhasmUtil Pseudo State.
+Require Export Wordize Vectorize.
+
+Module Conversion.
+  Import Pseudo ListNotations StateCommon EvalUtil ListState.
+
+  Hint Unfold setList getList getVar setCarry setCarryOpt getCarry
+       getMem setMem overflows.
+
+  Lemma pseudo_var: forall {w s n} x k v b p m c,
+      nth_error x k = Some v
+    -> pseudoEval (@PVar w s n b (exist _ k p)) (x, m, c) = Some ([v], m, c).
+  Proof.
+    intros; simpl; autounfold; simpl.
+    destruct (nth_error x k); simpl; try inversion H; intuition.
+  Qed.
+
+  Lemma pseudo_mem: forall {w s} n v m c x name len index p0 p1,
+      TripleM.find (w, name mod n, index mod len)%nat m = Some (@wordToN w v)
+    -> pseudoEval (@PMem w s n len (indexize _ p0 name) (indexize _ p1 index)) (x, m, c) = Some ([v], m, c).
+  Proof.
+    intros; autounfold; simpl.
+    unfold getMem; simpl.
+    rewrite H; autounfold; simpl.
+    rewrite NToWord_wordToN; intuition.
+  Qed.
+
+  Lemma pseudo_const: forall {w s n} x v m c,
+      pseudoEval (@PConst w s n v) (x, m, c) = Some ([v], m, c).
+  Proof. intros; simpl; intuition. Qed.
+
+  Lemma pseudo_plus:
+    forall {w s n} (p: @Pseudo w s n 2) x out0 out1 m0 m1 c0 c1,
+      pseudoEval p (x, m0, c0) = Some ([out0; out1], m1, c1)
+    -> pseudoEval (PBin n Add p) (x, m0, c0) =
+        Some ([out0 ^+ out1], m1,
+          Some (proj1_sig (bool_of_sumbool
+               (overflows w (&out0 + &out1)%N)%w))).
+  Proof.
+    intros; simpl; rewrite H; simpl.
+
+    pose proof (wordize_plus out0 out1).
+    destruct (overflows w _); autounfold; simpl; try rewrite H0;
+      try rewrite <- (@Npow2_ignore w (out0 ^+ out1));
+      try rewrite NToWord_wordToN; intuition.
+  Qed.
+
+  Lemma pseudo_bin:
+    forall {w s n} (p: @Pseudo w s n 2) x out0 out1 m0 m1 c0 c1 op,
+      op <> Add
+    -> pseudoEval p (x, m0, c0) = Some ([out0; out1], m1, c1)
+    -> pseudoEval (PBin n op p) (x, m0, c0) =
+        Some ([fst (evalIntOp op out0 out1)], m1, c1).
+  Proof.
+    intros; simpl; rewrite H0; simpl.
+
+    induction op;
+      try (contradict H; reflexivity);
+      unfold evalIntOp; autounfold; simpl;
+      reflexivity.
+  Qed.
+
+  Lemma pseudo_and:
+    forall {w s n} (p: @Pseudo w s n 2) x out0 out1 m0 m1 c0 c1,
+      pseudoEval p (x, m0, c0) = Some ([out0; out1], m1, c1)
+    -> pseudoEval (PBin n And p) (x, m0, c0) =
+        Some ([out0 ^& out1], m1, c1).
+  Proof.
+    intros.
+    replace (out0 ^& out1) with (fst (evalIntOp And out0 out1)).
+    - apply pseudo_bin; intuition; inversion H0.
+    - unfold evalIntOp; simpl; intuition.
+  Qed.
+
+  Lemma pseudo_awc:
+    forall {w s n} (p: @Pseudo w s n 2) x out0 out1 m0 m1 c0 c,
+      pseudoEval p (x, m0, c0) = Some ([out0; out1], m1, Some c)
+    -> pseudoEval (PCarry n AddWithCarry p) (x, m0, c0) =
+        Some ([addWithCarry out0 out1 c], m1,
+          Some (proj1_sig (bool_of_sumbool (overflows w
+          (&out0 + &out1 + (if c then 1 else 0))%N)%w))).
+  Proof.
+    intros; simpl; rewrite H; simpl.
+
+    pose proof (wordize_awc out0 out1); unfold evalCarryOp.
+    destruct (overflows w ((& out0)%w + (& out1)%w +
+                           (if c then 1%N else 0%N)));
+      autounfold; simpl; try rewrite H0; intuition.
+  Qed.
+
+  Lemma pseudo_shiftr:
+    forall {w s n} (p: @Pseudo w s n 1) x out m0 m1 c0 c1 k,
+      pseudoEval p (x, m0, c0) = Some ([out], m1, c1)
+    -> pseudoEval (PShift n Shr k p) (x, m0, c0) =
+        Some ([shiftr out k], m1, c1).
+  Proof.
+    intros; simpl; rewrite H; autounfold; simpl.
+    rewrite wordize_shiftr; rewrite NToWord_wordToN; intuition.
+  Qed.
+
+  Lemma pseudo_dual:
+    forall {w s n} (p: @Pseudo w s n 1) x out0 out1 m0 m1 c0 c1 k,
+      pseudoEval p (x, m0, c0) = Some ([out0; out1], m1, c1)
+    -> pseudoEval (PDual n Mult p) (x, m0, c0) =
+      Some ([x ^* y; (highBits (n/2) x) ^* (highBits (n/2) y)], m1, c1).
+  Proof.
+    intros; simpl; rewrite H; autounfold; simpl.
+    rewrite wordize_shiftr; rewrite NToWord_wordToN; intuition.
+  Qed.
+
+  Lemma pseudo_comb:
+    forall {w s n a b} (p0: @Pseudo w s n a) (p1: @Pseudo w s n b)
+      input out0 out1 m0 m1 m2 c0 c1 c2,
+      pseudoEval p0 (input, m0, c0) = Some (out0, m1, c1)
+    -> pseudoEval p1 (input, m1, c1) = Some (out1, m2, c2)
+    -> pseudoEval (@PComb w s n _ _ p0 p1) (input, m0, c0) =
+        Some (out0 ++ out1, m2, c2).
+  Proof.
+    intros; autounfold; simpl.
+    rewrite H; autounfold; simpl.
+    rewrite H0; autounfold; simpl; intuition.
+  Qed.
+
+  Lemma pseudo_cons:
+    forall {w s n b} (p0: @Pseudo w s n 1) (p1: @Pseudo w s n b)
+        (p2: @Pseudo w s n (S b)) input x xs m0 m1 m2 c0 c1 c2,
+      pseudoEval p0 (input, m0, c0) = Some ([x], m1, c1)
+    -> pseudoEval p1 (input, m1, c1) = Some (xs, m2, c2)
+    -> p2 = (@PComb w s n _ _ p0 p1)
+    -> pseudoEval p2 (input, m0, c0) = Some (x :: xs, m2, c2).
+  Proof.
+    intros.
+    replace (x :: xs) with ([x] ++ xs) by (simpl; intuition).
+    rewrite H1.
+    apply (pseudo_comb p0 p1 input _ _ m0 m1 m2 c0 c1 c2); intuition.
+  Qed.
+
+  Definition pseudeq {w s} (n m: nat) (f: list (word w) -> list (word w)) : Type := 
+    {p: @Pseudo w s n m | forall x: (list (word w)),
+      List.length x = n -> exists m' c',
+      pseudoEval p (x, TripleM.empty N, None) = Some (f x, m', c')}.
+
+  Definition example (v: list (word 32)) : list (word 32) :=
+      [(natToWord _ 1) ^& (nth 0 v (wzero _))].
+
+  Ltac autodestruct :=
+    repeat match goal with
+    | [H: context[Datatypes.length (cons _ _)] |- _] => simpl in H
+    | [H: context[Datatypes.length nil] |- _] => simpl in H
+    | [H: S ?a = S ?b |- _] => inversion H; clear H
+    | [H: (S ?a) = 0 |- _] => contradict H; intuition
+    | [H: 0 = (S ?a) |- _] => contradict H; intuition
+    | [H: 0 = 0 |- _] => clear H
+    | [x: list ?T |- _] =>
+      match goal with
+      | [H: context[Datatypes.length x] |- _] => destruct x
+      end
+    end.
+
+  Definition convert_example: @pseudeq 32 W32 1 1 example.
+    repeat eexists; unfold example; autounfold; autodestruct.
+
+    eapply pseudo_and.
+    eapply pseudo_cons.
+    eapply pseudo_const.
+    eapply pseudo_var.
+
+    (* leftovers *)
+
+    instantiate (1 := 0); simpl; intuition.
+    reflexivity.
+
+    Grab Existential Variables.
+
+    abstract (simpl; intuition).
+    exact None.
+  Defined.
+
+  Eval simpl in (proj1_sig convert_example).
+
+End Conversion.
+
